`PUSH0` opcode equivalence (#4)
* Create `Summaries` folder

* Add `StopSummary.lean`

* Update `AddSummary.lean`

* `AddEquivalence`: reflect `Sumaries` -> `AddSummary` change

* Add `Push0Summary.lean`

* Add `README.md` to `Summaries` folder

* Add `Interfaces/README.md`

* `Interfaces/README.md`: typo

* `Tactics.lean`: remove spurious comment

* Rename `_toNat` theorems

* Update generated Lean code to get the `PUSHZERO` summary

* Move theorems from `AddEquivalence` to `EvmYulInterface`

* `ScheduleOrdering.lean`: use namespaces

* Move theorems from `AddSummary` to `StopSummary`

* `StopSummary`: add `decode_singleton_stop`

* `Push0Summary.lean`: prove `X_push0_summary`

* `Push0Summary.lean`: optimize proofs

* Move `X_bad_pc` from `Push0Summary` to `EvmYulInterface`

* `Push0Summary`: more general `X_push0_summary`

* Correct symbolic stack lengths

* `AddSummary.lean`: Optimize `X_add_summary`

* Add `Equivalence` folder

* Add `Push0Equivalence.lean`

* `EvmYulInterface.lean`: add `add_succ_mod_size` theorem

* `AddEquivalence` optimize `step_add_equiv` with `add_suc_mod_size`

* `AddEquivalence`: remove spurious `_Val3` from `addRHS`

* `GasInterface`: add `simp` attribute to `cancun_def`

* `FuncInterface`: add `axiom ltInt_def`

* `Push0Summary`: explicit variables and `simp` attributes

* `Push0Equivalence`: prove equivalence for `push0` opcode

EvmEquivalence/Equivalence/Push0Equivalence.lean
@@ -1,4 +1,4 @@
-import EvmEquivalence.Summaries
+import EvmEquivalence.Summaries.Push0Summary
 import EvmEquivalence.StateMap
 import EvmEquivalence.Interfaces.FuncInterface
 import EvmEquivalence.Interfaces.GasInterface
@@ -6,12 +6,14 @@ import EvmEquivalence.Interfaces.EvmYulInterface
 
 open EvmYul
 open StateMap
+open GasInterface
 open KEVMInterface
+open Push0Summary
 
-namespace AddOpcodeEquivalence
+namespace Push0Equivalence
 
-def addLHS
-  {GAS_CELL PC_CELL W0 W1 : SortInt}
+def push0LHS
+  {GAS_CELL PC_CELL : SortInt}
   {K_CELL : SortK}
   {SCHEDULE_CELL : SortSchedule}
   {USEGAS_CELL : SortBool}
@@ -41,15 +43,14 @@ def addLHS
   {_Gen6 : SortLocalMemCell}
   {_Gen7 : SortMemoryUsedCell}
   {_Gen8 : SortCallGasCell}
-  {_Gen9 : SortStaticCell}
-  : SortGeneratedTopCell :=
+  {_Gen9 : SortStaticCell}: SortGeneratedTopCell :=
   { kevm := {
-      k := { val := SortK.kseq ((@inj SortInternalOp SortKItem) (SortInternalOp.«#next[_]_EVM_InternalOp_MaybeOpCode» ((@inj SortBinStackOp   SortMaybeOpCode) SortBinStackOp.ADD_EVM_BinStackOp))) K_CELL },
-      exitCode := _Gen22,
-      mode := _Gen23,
-      schedule := { val := SCHEDULE_CELL },
-      useGas := { val := USEGAS_CELL },
-      ethereum := {
+    k := { val := SortK.kseq ((@inj SortInternalOp SortKItem) (SortInternalOp.«#next[_]_EVM_InternalOp_MaybeOpCode» ((@inj SortPushOp SortMaybeOpCode) SortPushOp.PUSHZERO_EVM_PushOp))) K_CELL },
+    exitCode := _Gen22,
+    mode := _Gen23,
+    schedule := { val := SCHEDULE_CELL },
+    useGas := { val := USEGAS_CELL },
+    ethereum := {
       evm := {
         output := _Gen11,
         statusCode := _Gen12,
@@ -63,8 +64,7 @@ def addLHS
           caller := _Gen3,
           callData := _Gen4,
           callValue := _Gen5,
-          wordStack := { val :=
-            SortWordStack.«_:__EVM-TYPES_WordStack_Int_WordStack» W0        (SortWordStack.«_:__EVM-TYPES_WordStack_Int_WordStack» W1 WS) },
+          wordStack := { val := WS },
           localMem := _Gen6,
           pc := { val := PC_CELL },
           gas := { val := (@inj SortInt SortGas) GAS_CELL },
@@ -81,8 +81,8 @@ def addLHS
       network := _DotVar2 } },
     generatedCounter := _DotVar0 }
 
-def addRHS
-  {_Val0 _Val1 _Val2 _Val3 _Val4 : SortInt}
+def push0RHS
+  {_Val10 _Val8 : SortInt}
   {K_CELL : SortK}
   {SCHEDULE_CELL : SortSchedule}
   {WS : SortWordStack}
@@ -111,8 +111,7 @@ def addRHS
   {_Gen6 : SortLocalMemCell}
   {_Gen7 : SortMemoryUsedCell}
   {_Gen8 : SortCallGasCell}
-  {_Gen9 : SortStaticCell}
-  : SortGeneratedTopCell :=
+  {_Gen9 : SortStaticCell}: SortGeneratedTopCell :=
   { kevm := {
     k := { val := K_CELL },
     exitCode := _Gen22,
@@ -133,10 +132,10 @@ def addRHS
           caller := _Gen3,
           callData := _Gen4,
           callValue := _Gen5,
-          wordStack := { val := SortWordStack.«_:__EVM-TYPES_WordStack_Int_WordStack» _Val1 WS },
+          wordStack := { val := SortWordStack.«_:__EVM-TYPES_WordStack_Int_WordStack» 0 WS },
           localMem := _Gen6,
-          pc := { val := _Val2 },
-          gas := { val := (@inj SortInt SortGas) _Val4 },
+          pc := { val := _Val8 },
+          gas := { val := (@inj SortInt SortGas) _Val10 },
           memoryUsed := _Gen7,
           callGas := _Gen8,
           static := _Gen9,
@@ -150,11 +149,11 @@ def addRHS
       network := _DotVar2 } },
     generatedCounter := _DotVar0 }
 
-theorem rw_addLHS_addRHS
-  {GAS_CELL PC_CELL W0 W1 _Val0 _Val1 _Val2 _Val3 _Val4 : SortInt}
+theorem rw_push0LHS_push0RHS
+  {GAS_CELL PC_CELL _Val0 _Val10 _Val3 _Val8 _Val9 : SortInt}
   {K_CELL : SortK}
   {SCHEDULE_CELL : SortSchedule}
-  {USEGAS_CELL : SortBool}
+  {USEGAS_CELL _Val1 _Val2 _Val4 _Val5 _Val6 _Val7 : SortBool}
   {WS : SortWordStack}
   {_DotVar0 : SortGeneratedCounterCell}
   {_DotVar2 : SortNetworkCell}
@@ -182,19 +181,26 @@ theorem rw_addLHS_addRHS
   {_Gen7 : SortMemoryUsedCell}
   {_Gen8 : SortCallGasCell}
   {_Gen9 : SortStaticCell}
-  (defn_Val0 : «_+Int_» W0 W1 = some _Val0)
-  (defn_Val1 : chop _Val0 = some _Val1)
-  (defn_Val2 : «_+Int_» PC_CELL 1 = some _Val2)
-  (defn_Val3 : «_<_>_SCHEDULE_Int_ScheduleConst_Schedule» SortScheduleConst.Gverylow_SCHEDULE_ScheduleConst SCHEDULE_CELL = some _Val3)
-  (defn_Val4 : «_-Int_» GAS_CELL _Val3 = some _Val4)
-  (req : USEGAS_CELL = true):
+  (defn_Val0 : sizeWordStackAux WS 0 = some _Val0)
+  (defn_Val1 : «_<Int_» _Val0 0 = some _Val1)
+  (defn_Val2 : notBool_ _Val1 = some _Val2)
+  (defn_Val3 : sizeWordStackAux WS 0 = some _Val3)
+  (defn_Val4 : «_<Int_» 1023 _Val3 = some _Val4)
+  (defn_Val5 : notBool_ _Val4 = some _Val5)
+  (defn_Val6 : _andBool_ _Val2 _Val5 = some _Val6)
+  (defn_Val7 : _andBool_ USEGAS_CELL _Val6 = some _Val7)
+  (defn_Val8 : «_+Int_» PC_CELL 1 = some _Val8)
+  (defn_Val9 : «_<_>_SCHEDULE_Int_ScheduleConst_Schedule» SortScheduleConst.Gbase_SCHEDULE_ScheduleConst SCHEDULE_CELL = some _Val9)
+  (defn_Val10 : «_-Int_» GAS_CELL _Val9 = some _Val10)
+  (req : _Val7 = true):
   Rewrites
-    (@addLHS GAS_CELL PC_CELL W0 W1 K_CELL SCHEDULE_CELL USEGAS_CELL WS _DotVar0 _DotVar2 _Gen0 _Gen1 _Gen10 _Gen11 _Gen12 _Gen13 _Gen14 _Gen15 _Gen16 _Gen17 _Gen18 _Gen19 _Gen2 _Gen20 _Gen21 _Gen22 _Gen23 _Gen3 _Gen4 _Gen5 _Gen6 _Gen7 _Gen8 _Gen9)
-    (@addRHS _Val0 _Val1 _Val2 _Val3 _Val4 K_CELL SCHEDULE_CELL WS _DotVar0 _DotVar2 _Gen0 _Gen1 _Gen10 _Gen11 _Gen12 _Gen13 _Gen14 _Gen15 _Gen16 _Gen17 _Gen18 _Gen19 _Gen2 _Gen20 _Gen21 _Gen22 _Gen23 _Gen3 _Gen4 _Gen5 _Gen6 _Gen7 _Gen8 _Gen9) := by
-  apply Rewrites.SUMMARY_ADD_2_SPEC_BASIC_BLOCK_8_TO_6 <;> try assumption
+  (@push0LHS GAS_CELL PC_CELL K_CELL SCHEDULE_CELL USEGAS_CELL WS _DotVar0 _DotVar2 _Gen0 _Gen1 _Gen10 _Gen11 _Gen12 _Gen13 _Gen14 _Gen15 _Gen16 _Gen17 _Gen18 _Gen19 _Gen2 _Gen20 _Gen21 _Gen22 _Gen23 _Gen3 _Gen4 _Gen5 _Gen6 _Gen7 _Gen8 _Gen9)
+  (@push0RHS _Val10 _Val8 K_CELL SCHEDULE_CELL WS _DotVar0 _DotVar2 _Gen0 _Gen1 _Gen10 _Gen11 _Gen12 _Gen13 _Gen14 _Gen15 _Gen16 _Gen17 _Gen18 _Gen19 _Gen2 _Gen20 _Gen21 _Gen22 _Gen23 _Gen3 _Gen4 _Gen5 _Gen6 _Gen7 _Gen8 _Gen9) :=
+  by apply Rewrites.SUMMARY_PUSHZERO_0_SPEC_BASIC_BLOCK_11_TO_9 <;> try assumption
+     all_goals simp_all [notBool_def, andBool_def]
 
-theorem add_prestate_equiv
-  {GAS_CELL PC_CELL W0 W1 _Val0 _Val1 _Val2 _Val3 _Val4 : SortInt}
+theorem push0_prestate_equiv
+  {GAS_CELL PC_CELL : SortInt}
   {K_CELL : SortK}
   {SCHEDULE_CELL : SortSchedule}
   {USEGAS_CELL : SortBool}
@@ -225,18 +231,19 @@ theorem add_prestate_equiv
   {_Gen7 : SortMemoryUsedCell}
   {_Gen8 : SortCallGasCell}
   {_Gen9 : SortStaticCell}
-  (symState : EVM.State):
-  stateMap symState (@addLHS GAS_CELL PC_CELL W0 W1 K_CELL SCHEDULE_CELL USEGAS_CELL WS _DotVar0 _DotVar2 _Gen0 _Gen1 _Gen10 _Gen11 _Gen12 _Gen13 _Gen14 _Gen15 _Gen16 _Gen17 _Gen18 _Gen19 _Gen2 _Gen20 _Gen21 _Gen22 _Gen23 _Gen3 _Gen4 _Gen5 _Gen6 _Gen7 _Gen8 _Gen9) =
+  {symState : EVM.State}:
+  stateMap symState (@push0LHS GAS_CELL PC_CELL K_CELL SCHEDULE_CELL USEGAS_CELL WS _DotVar0 _DotVar2 _Gen0 _Gen1 _Gen10 _Gen11 _Gen12 _Gen13 _Gen14 _Gen15 _Gen16 _Gen17 _Gen18 _Gen19 _Gen2 _Gen20 _Gen21 _Gen22 _Gen23 _Gen3 _Gen4 _Gen5 _Gen6 _Gen7 _Gen8 _Gen9) =
   {symState with
-    stack := (intMap W0) :: (intMap W1) :: wordStackMap WS
+    stack := wordStackMap WS
     pc := intMap PC_CELL
     gasAvailable := intMap GAS_CELL
     executionEnv := {symState.executionEnv with code := _Gen0.val}
     returnData := _Gen11.val
     } := rfl
 
-theorem add_poststate_equiv
-  {PC_CELL W0 W1 _Val0 _Val1 _Val2 _Val3 _Val4 : SortInt}
+theorem push0_poststate_equiv
+  (PC_CELL : SortInt)
+  {_Val10 _Val8 : SortInt}
   {K_CELL : SortK}
   {SCHEDULE_CELL : SortSchedule}
   {WS : SortWordStack}
@@ -266,28 +273,22 @@ theorem add_poststate_equiv
   {_Gen7 : SortMemoryUsedCell}
   {_Gen8 : SortCallGasCell}
   {_Gen9 : SortStaticCell}
-  (defn_Val0 : «_+Int_» W0 W1 = some _Val0)
-  (defn_Val1 : chop _Val0 = some _Val1)
-  (defn_Val2 : «_+Int_» PC_CELL 1 = some _Val2)
-  (symState : EVM.State):
-  stateMap symState (@addRHS _Val0 _Val1 _Val2 _Val3 _Val4 K_CELL SCHEDULE_CELL WS _DotVar0 _DotVar2 _Gen0 _Gen1 _Gen10 _Gen11 _Gen12 _Gen13 _Gen14 _Gen15 _Gen16 _Gen17 _Gen18 _Gen19 _Gen2 _Gen20 _Gen21 _Gen22 _Gen23 _Gen3 _Gen4 _Gen5 _Gen6 _Gen7 _Gen8 _Gen9) =
+  {symState : EVM.State}
+  (defn_Val8 : «_+Int_» PC_CELL 1 = some _Val8):
+  stateMap symState (@push0RHS _Val10 _Val8 K_CELL SCHEDULE_CELL WS _DotVar0 _DotVar2 _Gen0 _Gen1 _Gen10 _Gen11 _Gen12 _Gen13 _Gen14 _Gen15 _Gen16 _Gen17 _Gen18 _Gen19 _Gen2 _Gen20 _Gen21 _Gen22 _Gen23 _Gen3 _Gen4 _Gen5 _Gen6 _Gen7 _Gen8 _Gen9) =
   {symState with
-    stack := (intMap (chop' («_+Int'_» W0 W1))) :: wordStackMap WS
+    stack := .ofNat 0 :: wordStackMap WS
     pc := intMap («_+Int'_» PC_CELL 1)
-    gasAvailable := intMap _Val4
+    gasAvailable := intMap _Val10
     executionEnv := {symState.executionEnv with code := _Gen0.val}
     returnData := _Gen11.val
-    } := by aesop (add simp [«_+Int'_», chop'])
+    } := by aesop (add simp [«_+Int'_»])
 
-open AddSummary
-
--- We cannot prove full equivalence for the `EVM.step` function
--- This is because it doesn't include all semantics such as gas computation
-theorem step_add_equiv
-  {GAS_CELL PC_CELL W0 W1 _Val0 _Val1 _Val2 _Val3 _Val4 : SortInt}
+theorem step_push0_equiv
+  {GAS_CELL PC_CELL _Val0 _Val10 _Val3 _Val8 _Val9 : SortInt}
   {K_CELL : SortK}
   {SCHEDULE_CELL : SortSchedule}
-  {USEGAS_CELL : SortBool}
+  {USEGAS_CELL _Val1 _Val2 _Val4 _Val5 _Val6 _Val7 : SortBool}
   {WS : SortWordStack}
   {_DotVar0 : SortGeneratedCounterCell}
   {_DotVar2 : SortNetworkCell}
@@ -315,53 +316,46 @@ theorem step_add_equiv
   {_Gen7 : SortMemoryUsedCell}
   {_Gen8 : SortCallGasCell}
   {_Gen9 : SortStaticCell}
-  (defn_Val0 : «_+Int_» W0 W1 = some _Val0)
-  (defn_Val1 : chop _Val0 = some _Val1)
-  (defn_Val2 : «_+Int_» PC_CELL 1 = some _Val2)
-  (defn_Val3 : «_<_>_SCHEDULE_Int_ScheduleConst_Schedule» SortScheduleConst.Gverylow_SCHEDULE_ScheduleConst SCHEDULE_CELL = some _Val3)
-  (defn_Val4 : «_-Int_» GAS_CELL _Val3 = some _Val4)
-  (symState : EVM.State)
+  {symState : EVM.State}
+  (defn_Val0 : sizeWordStackAux WS 0 = some _Val0)
+  (defn_Val1 : «_<Int_» _Val0 0 = some _Val1)
+  (defn_Val2 : notBool_ _Val1 = some _Val2)
+  (defn_Val3 : sizeWordStackAux WS 0 = some _Val3)
+  (defn_Val4 : «_<Int_» 1023 _Val3 = some _Val4)
+  (defn_Val5 : notBool_ _Val4 = some _Val5)
+  (defn_Val6 : _andBool_ _Val2 _Val5 = some _Val6)
+  (defn_Val7 : _andBool_ USEGAS_CELL _Val6 = some _Val7)
+  (defn_Val8 : «_+Int_» PC_CELL 1 = some _Val8)
+  (defn_Val9 : «_<_>_SCHEDULE_Int_ScheduleConst_Schedule» SortScheduleConst.Gbase_SCHEDULE_ScheduleConst SCHEDULE_CELL = some _Val9)
+  (defn_Val10 : «_-Int_» GAS_CELL _Val9 = some _Val10)
+  (req : _Val7 = true)
   -- needed for EVM.step
   (gas gasCost : ℕ)
   -- Necessary assumptions for equivalence
   (cancun : SCHEDULE_CELL = .CANCUN_EVM)
   (gasEnough : 0 < gas)
-  (gavailEnough : 3 ≤ GAS_CELL)
+  (gavailEnough : 2 ≤ GAS_CELL)
   (gavailSmall : GAS_CELL < ↑UInt256.size)
-  (gasCostValue : gasCost = GasConstants.Gverylow)
+  (gasCostValue : gasCost = GasConstants.Gbase)
   (pcountSmall : PC_CELL + 1 < UInt256.size)
-  (pcountNonneg : 0 ≤ PC_CELL)
-  (W0ge0 : 0 ≤ W0)
-  (W1ge0 : 0 ≤ W1):
-  EVM.step_add gas gasCost (stateMap symState (@addLHS GAS_CELL PC_CELL W0 W1 K_CELL SCHEDULE_CELL USEGAS_CELL WS _DotVar0 _DotVar2 _Gen0 _Gen1 _Gen10 _Gen11 _Gen12 _Gen13 _Gen14 _Gen15 _Gen16 _Gen17 _Gen18 _Gen19 _Gen2 _Gen20 _Gen21 _Gen22 _Gen23 _Gen3 _Gen4 _Gen5 _Gen6 _Gen7 _Gen8 _Gen9)) =
-  .ok (stateMap {symState with execLength := symState.execLength + 1} (@addRHS _Val0 _Val1 _Val2 _Val3 _Val4 K_CELL SCHEDULE_CELL WS _DotVar0 _DotVar2 _Gen0 _Gen1 _Gen10 _Gen11 _Gen12 _Gen13 _Gen14 _Gen15 _Gen16 _Gen17 _Gen18 _Gen19 _Gen2 _Gen20 _Gen21 _Gen22 _Gen23 _Gen3 _Gen4 _Gen5 _Gen6 _Gen7 _Gen8 _Gen9)) := by
-  rw [add_prestate_equiv, add_poststate_equiv] <;> try assumption
+  (pcountNonneg : 0 ≤ PC_CELL):
+  EVM.step_push0 gas gasCost (stateMap symState (@push0LHS GAS_CELL PC_CELL K_CELL SCHEDULE_CELL USEGAS_CELL WS _DotVar0 _DotVar2 _Gen0 _Gen1 _Gen10 _Gen11 _Gen12 _Gen13 _Gen14 _Gen15 _Gen16 _Gen17 _Gen18 _Gen19 _Gen2 _Gen20 _Gen21 _Gen22 _Gen23 _Gen3 _Gen4 _Gen5 _Gen6 _Gen7 _Gen8 _Gen9)) =
+  .ok (stateMap {symState with execLength := symState.execLength + 1} (@push0RHS _Val10 _Val8 K_CELL SCHEDULE_CELL WS _DotVar0 _DotVar2 _Gen0 _Gen1 _Gen10 _Gen11 _Gen12 _Gen13 _Gen14 _Gen15 _Gen16 _Gen17 _Gen18 _Gen19 _Gen2 _Gen20 _Gen21 _Gen22 _Gen23 _Gen3 _Gen4 _Gen5 _Gen6 _Gen7 _Gen8 _Gen9)) := by
+  rw [push0_prestate_equiv, (push0_poststate_equiv PC_CELL)]
   cases gas; contradiction
-  case succ gas =>
-    rw [EVM.step_add_summary] <;> try assumption
-    congr
-    . aesop (add simp [GasInterface.cancun_def, «_-Int_»])
-            (add simp [intMap_sub_dist])
-    . have mod_rw : (PC_CELL + 1) % UInt256.size = PC_CELL + 1 := by
-        rw [Int.mod_cast, Int.toNat_ofNat, Nat.mod_eq_of_lt] <;> try linarith
-        . aesop (add safe (by linarith))
-        . rw [Int.toNat_lt] <;> linarith
-      rw [plusInt_def, ←mod_rw, intMap_add_dist] <;> aesop
-    . aesop (add simp [intMap, chop_def, plusInt_def, intMap_add_dist])
+  rw [EVM.step_push0_summary] <;> try assumption
+  congr
+  . aesop (add simp [GasConstants.Gbase, «_-Int_», cancun_def, intMap_sub_dist])
+  . rw [plusInt_def, ←UInt256.add_succ_mod_size, intMap_add_dist] <;> aesop
+  . aesop (add simp [«_+Int_»])
 
-/- Deviations from the KEVM produced specifications:
- 1. The program is not symbolic, it is instead a 1-opcode (`ADD`) program
- 2. The program counter is also not symbolic, and it is set to 0
- 3. In the RHS, the output cell (mapped to `returnData`) is set to `ByteArray.empty`
- 4. The schedule is set to `CANCUN`
- 5. `GAVAIL` is in the `UInt256` range
- 6. `W0` and `W1` are nonnegative
- -/
-theorem X_add_equiv
-  {GAS_CELL PC_CELL W0 W1 _Val0 _Val1 _Val2 _Val3 _Val4 : SortInt}
+attribute [local simp] GasConstants.Gbase
+
+theorem X_push0_equiv
+  {GAS_CELL PC_CELL _Val0 _Val10 _Val3 _Val8 _Val9 : SortInt}
   {K_CELL : SortK}
   {SCHEDULE_CELL : SortSchedule}
-  {USEGAS_CELL : SortBool}
+  {USEGAS_CELL _Val1 _Val2 _Val4 _Val5 _Val6 _Val7 : SortBool}
   {WS : SortWordStack}
   {_DotVar0 : SortGeneratedCounterCell}
   {_DotVar2 : SortNetworkCell}
@@ -389,36 +383,42 @@ theorem X_add_equiv
   {_Gen7 : SortMemoryUsedCell}
   {_Gen8 : SortCallGasCell}
   {_Gen9 : SortStaticCell}
-  (defn_Val0 : «_+Int_» W0 W1 = some _Val0)
-  (defn_Val1 : chop _Val0 = some _Val1)
-  (defn_Val2 : «_+Int_» PC_CELL 1 = some _Val2)
-  (defn_Val3 : «_<_>_SCHEDULE_Int_ScheduleConst_Schedule» SortScheduleConst.Gverylow_SCHEDULE_ScheduleConst SCHEDULE_CELL = some _Val3)
-  (defn_Val4 : «_-Int_» GAS_CELL _Val3 = some _Val4)
-  (symState : EVM.State)
+  {symState : EVM.State}
+  (defn_Val0 : sizeWordStackAux WS 0 = some _Val0)
+  (defn_Val1 : «_<Int_» _Val0 0 = some _Val1)
+  --(defn_Val2 : notBool_ _Val1 = some _Val2)
+  (defn_Val3 : sizeWordStackAux WS 0 = some _Val3)
+  (defn_Val4 : «_<Int_» 1023 _Val3 = some _Val4)
+  (defn_Val5 : notBool_ _Val4 = some _Val5)
+  (defn_Val6 : _andBool_ _Val2 _Val5 = some _Val6)
+  (defn_Val7 : _andBool_ USEGAS_CELL _Val6 = some _Val7)
+  (defn_Val8 : «_+Int_» PC_CELL 1 = some _Val8)
+  (defn_Val9 : «_<_>_SCHEDULE_Int_ScheduleConst_Schedule» SortScheduleConst.Gbase_SCHEDULE_ScheduleConst SCHEDULE_CELL = some _Val9)
+  (defn_Val10 : «_-Int_» GAS_CELL _Val9 = some _Val10)
+  (req : _Val7 = true)
   -- Necessary assumptions for equivalence
   (cancun : SCHEDULE_CELL = .CANCUN_EVM)
-  (codeAdd : _Gen0 = ⟨⟨#[(1 : UInt8)]⟩⟩)
+  --(gasEnough : 0 < gas)
+  (gavailEnough : 2 < GAS_CELL)
+  (gavailSmall : GAS_CELL < ↑UInt256.size)
+  (pcountSmall : PC_CELL + 1 < UInt256.size)
+  (pcountNonneg : 0 ≤ PC_CELL)
+  -- Specific to executing a 1-opcode program
+  (codePush0 : _Gen0 = ⟨⟨#[(0x5F : UInt8)]⟩⟩)
   (pcZero : PC_CELL = 0)
-  (enoughGas : 3 < GAS_CELL)
-  (boundedGas : GAS_CELL < ↑UInt256.size)
-  (W0ge0 : 0 ≤ W0)
-  (W1ge0 : 0 ≤ W1)
-  -- There's no #sizeWordStack
-  (wordStackOk : sizeWordStackAux WS 0 < some 1024):
-  EVM.X false (UInt256.toNat (intMap GAS_CELL)) (stateMap symState (@addLHS GAS_CELL PC_CELL W0 W1 K_CELL SCHEDULE_CELL USEGAS_CELL WS _DotVar0 _DotVar2 _Gen0 _Gen1 _Gen10 _Gen11 _Gen12 _Gen13 _Gen14 _Gen15 _Gen16 _Gen17 _Gen18 _Gen19 _Gen2 _Gen20 _Gen21 _Gen22 _Gen23 _Gen3 _Gen4 _Gen5 _Gen6 _Gen7 _Gen8 _Gen9)) =
-  .ok (.success (stateMap {symState with execLength := symState.execLength + 2} (@addRHS _Val0 _Val1 _Val2 _Val3 _Val4 K_CELL SCHEDULE_CELL WS _DotVar0 _DotVar2 _Gen0 _Gen1 _Gen10 ⟨ByteArray.empty⟩ _Gen12 _Gen13 _Gen14 _Gen15 _Gen16 _Gen17 _Gen18 _Gen19 _Gen2 _Gen20 _Gen21 _Gen22 _Gen23 _Gen3 _Gen4 _Gen5 _Gen6 _Gen7 _Gen8 _Gen9)) ByteArray.empty) := by
-  -- With `simp` doesn't work
-  rw [codeAdd, pcZero, add_prestate_equiv, add_poststate_equiv] <;> try assumption
-  -- If we don't apply this lemma we cannot rewrite X_add_summary
-  have pc_equiv : intMap 0 = UInt256.ofNat 0 := rfl
-  rw [pc_equiv, X_add_summary]
-  · aesop (add simp [GasInterface.cancun_def, «_-Int_», chop_def, plusInt_def, intMap_add_dist])
-      (add safe (by rw [intMap_sub_dist])) (add safe (by apply le_of_lt))
-  · aesop (add simp [GasConstants.Gverylow, intMap, UInt256.toSigned])
-      (add simp [intMap_toNat_small, UInt256.ofNat_toNat])
-      (add safe (by contradiction))
-  · simp_all [sizeWordStack_def]
-    simp [LT.lt, Option.lt, OfNat.ofNat, (@Int.ofNat_eq_coe 1024)] at wordStackOk
-    exact (Int.lt_of_ofNat_lt_ofNat wordStackOk)
+  (returnEmpty : _Gen11 = ⟨ByteArray.empty⟩):
+  EVM.X false (UInt256.toNat (intMap GAS_CELL)) (stateMap symState (@push0LHS GAS_CELL PC_CELL K_CELL SCHEDULE_CELL USEGAS_CELL WS _DotVar0 _DotVar2 _Gen0 _Gen1 _Gen10 _Gen11 _Gen12 _Gen13 _Gen14 _Gen15 _Gen16 _Gen17 _Gen18 _Gen19 _Gen2 _Gen20 _Gen21 _Gen22 _Gen23 _Gen3 _Gen4 _Gen5 _Gen6 _Gen7 _Gen8 _Gen9)) =
+  .ok (.success (stateMap {symState with execLength := symState.execLength + 2} (@push0RHS _Val10 _Val8 K_CELL SCHEDULE_CELL WS _DotVar0 _DotVar2 _Gen0 _Gen1 _Gen10 _Gen11 _Gen12 _Gen13 _Gen14 _Gen15 _Gen16 _Gen17 _Gen18 _Gen19 _Gen2 _Gen20 _Gen21 _Gen22 _Gen23 _Gen3 _Gen4 _Gen5 _Gen6 _Gen7 _Gen8 _Gen9)) ByteArray.empty) := by
+  rw [codePush0, pcZero, push0_prestate_equiv, (push0_poststate_equiv PC_CELL)] <;> try assumption
+  rw [intMap_toNat] <;> first | linarith | try assumption
+  cases cgc: (UInt256.toNat (intMap GAS_CELL))
+  . rw [intMap_toNat, Int.toNat_eq_zero] at cgc <;> linarith
+  . have pc_equiv : intMap 0 = UInt256.ofNat 0 := rfl
+    rw [pc_equiv, ←intMap_toNat, X_push0_summary] <;> first | linarith | try simp
+    . aesop (add simp [«_-Int_», intMap_sub_dist])
+      (add safe (by rw [intMap_sub_dist])) (add safe (by linarith))
+    . rw [intMap_toNat] <;> aesop (add safe (by linarith))
+    . revert defn_Val4; simp_all [sizeWordStack_def, andBool_def, notBool_def,  ltInt_def]
+      aesop (add safe (by linarith))
 
-end AddOpcodeEquivalence
+end Push0Equivalence
