EvmEquivalence/Equivalence/AddEquivalence.lean
@@ -1,0 +1,419 @@
+import EvmEquivalence.Summaries.AddSummary
+import EvmEquivalence.StateMap
+import EvmEquivalence.Interfaces.FuncInterface
+import EvmEquivalence.Interfaces.GasInterface
+import EvmEquivalence.Interfaces.EvmYulInterface
+
+open EvmYul
+open StateMap
+open KEVMInterface
+
+namespace AddOpcodeEquivalence
+
+def addLHS
+  {GAS_CELL PC_CELL W0 W1 : SortInt}
+  {K_CELL : SortK}
+  {SCHEDULE_CELL : SortSchedule}
+  {USEGAS_CELL : SortBool}
+  {WS : SortWordStack}
+  {_DotVar0 : SortGeneratedCounterCell}
+  {_DotVar2 : SortNetworkCell}
+  {_Gen0 : SortProgramCell}
+  {_Gen1 : SortJumpDestsCell}
+  {_Gen10 : SortCallDepthCell}
+  {_Gen11 : SortOutputCell}
+  {_Gen12 : SortStatusCodeCell}
+  {_Gen13 : SortCallStackCell}
+  {_Gen14 : SortInterimStatesCell}
+  {_Gen15 : SortTouchedAccountsCell}
+  {_Gen16 : SortVersionedHashesCell}
+  {_Gen17 : SortSubstateCell}
+  {_Gen18 : SortGasPriceCell}
+  {_Gen19 : SortOriginCell}
+  {_Gen2 : SortIdCell}
+  {_Gen20 : SortBlockhashesCell}
+  {_Gen21 : SortBlockCell}
+  {_Gen22 : SortExitCodeCell}
+  {_Gen23 : SortModeCell}
+  {_Gen3 : SortCallerCell}
+  {_Gen4 : SortCallDataCell}
+  {_Gen5 : SortCallValueCell}
+  {_Gen6 : SortLocalMemCell}
+  {_Gen7 : SortMemoryUsedCell}
+  {_Gen8 : SortCallGasCell}
+  {_Gen9 : SortStaticCell}
+  : SortGeneratedTopCell :=
+  { kevm := {
+      k := { val := SortK.kseq ((@inj SortInternalOp SortKItem) (SortInternalOp.«#next[_]_EVM_InternalOp_MaybeOpCode» ((@inj SortBinStackOp   SortMaybeOpCode) SortBinStackOp.ADD_EVM_BinStackOp))) K_CELL },
+      exitCode := _Gen22,
+      mode := _Gen23,
+      schedule := { val := SCHEDULE_CELL },
+      useGas := { val := USEGAS_CELL },
+      ethereum := {
+      evm := {
+        output := _Gen11,
+        statusCode := _Gen12,
+        callStack := _Gen13,
+        interimStates := _Gen14,
+        touchedAccounts := _Gen15,
+        callState := {
+          program := _Gen0,
+          jumpDests := _Gen1,
+          id := _Gen2,
+          caller := _Gen3,
+          callData := _Gen4,
+          callValue := _Gen5,
+          wordStack := { val :=
+            SortWordStack.«_:__EVM-TYPES_WordStack_Int_WordStack» W0        (SortWordStack.«_:__EVM-TYPES_WordStack_Int_WordStack» W1 WS) },
+          localMem := _Gen6,
+          pc := { val := PC_CELL },
+          gas := { val := (@inj SortInt SortGas) GAS_CELL },
+          memoryUsed := _Gen7,
+          callGas := _Gen8,
+          static := _Gen9,
+          callDepth := _Gen10 },
+        versionedHashes := _Gen16,
+        substate := _Gen17,
+        gasPrice := _Gen18,
+        origin := _Gen19,
+        blockhashes := _Gen20,
+        block := _Gen21 },
+      network := _DotVar2 } },
+    generatedCounter := _DotVar0 }
+
+def addRHS
+  {_Val0 _Val1 _Val2 _Val4 : SortInt}
+  {K_CELL : SortK}
+  {SCHEDULE_CELL : SortSchedule}
+  {WS : SortWordStack}
+  {_DotVar0 : SortGeneratedCounterCell}
+  {_DotVar2 : SortNetworkCell}
+  {_Gen0 : SortProgramCell}
+  {_Gen1 : SortJumpDestsCell}
+  {_Gen10 : SortCallDepthCell}
+  {_Gen11 : SortOutputCell}
+  {_Gen12 : SortStatusCodeCell}
+  {_Gen13 : SortCallStackCell}
+  {_Gen14 : SortInterimStatesCell}
+  {_Gen15 : SortTouchedAccountsCell}
+  {_Gen16 : SortVersionedHashesCell}
+  {_Gen17 : SortSubstateCell}
+  {_Gen18 : SortGasPriceCell}
+  {_Gen19 : SortOriginCell}
+  {_Gen2 : SortIdCell}
+  {_Gen20 : SortBlockhashesCell}
+  {_Gen21 : SortBlockCell}
+  {_Gen22 : SortExitCodeCell}
+  {_Gen23 : SortModeCell}
+  {_Gen3 : SortCallerCell}
+  {_Gen4 : SortCallDataCell}
+  {_Gen5 : SortCallValueCell}
+  {_Gen6 : SortLocalMemCell}
+  {_Gen7 : SortMemoryUsedCell}
+  {_Gen8 : SortCallGasCell}
+  {_Gen9 : SortStaticCell}
+  : SortGeneratedTopCell :=
+  { kevm := {
+    k := { val := K_CELL },
+    exitCode := _Gen22,
+    mode := _Gen23,
+    schedule := { val := SCHEDULE_CELL },
+    useGas := { val := true },
+    ethereum := {
+      evm := {
+        output := _Gen11,
+        statusCode := _Gen12,
+        callStack := _Gen13,
+        interimStates := _Gen14,
+        touchedAccounts := _Gen15,
+        callState := {
+          program := _Gen0,
+          jumpDests := _Gen1,
+          id := _Gen2,
+          caller := _Gen3,
+          callData := _Gen4,
+          callValue := _Gen5,
+          wordStack := { val := SortWordStack.«_:__EVM-TYPES_WordStack_Int_WordStack» _Val1 WS },
+          localMem := _Gen6,
+          pc := { val := _Val2 },
+          gas := { val := (@inj SortInt SortGas) _Val4 },
+          memoryUsed := _Gen7,
+          callGas := _Gen8,
+          static := _Gen9,
+          callDepth := _Gen10 },
+        versionedHashes := _Gen16,
+        substate := _Gen17,
+        gasPrice := _Gen18,
+        origin := _Gen19,
+        blockhashes := _Gen20,
+        block := _Gen21 },
+      network := _DotVar2 } },
+    generatedCounter := _DotVar0 }
+
+theorem rw_addLHS_addRHS
+  {GAS_CELL PC_CELL W0 W1 _Val0 _Val1 _Val2 _Val3 _Val4 : SortInt}
+  {K_CELL : SortK}
+  {SCHEDULE_CELL : SortSchedule}
+  {USEGAS_CELL : SortBool}
+  {WS : SortWordStack}
+  {_DotVar0 : SortGeneratedCounterCell}
+  {_DotVar2 : SortNetworkCell}
+  {_Gen0 : SortProgramCell}
+  {_Gen1 : SortJumpDestsCell}
+  {_Gen10 : SortCallDepthCell}
+  {_Gen11 : SortOutputCell}
+  {_Gen12 : SortStatusCodeCell}
+  {_Gen13 : SortCallStackCell}
+  {_Gen14 : SortInterimStatesCell}
+  {_Gen15 : SortTouchedAccountsCell}
+  {_Gen16 : SortVersionedHashesCell}
+  {_Gen17 : SortSubstateCell}
+  {_Gen18 : SortGasPriceCell}
+  {_Gen19 : SortOriginCell}
+  {_Gen2 : SortIdCell}
+  {_Gen20 : SortBlockhashesCell}
+  {_Gen21 : SortBlockCell}
+  {_Gen22 : SortExitCodeCell}
+  {_Gen23 : SortModeCell}
+  {_Gen3 : SortCallerCell}
+  {_Gen4 : SortCallDataCell}
+  {_Gen5 : SortCallValueCell}
+  {_Gen6 : SortLocalMemCell}
+  {_Gen7 : SortMemoryUsedCell}
+  {_Gen8 : SortCallGasCell}
+  {_Gen9 : SortStaticCell}
+  (defn_Val0 : «_+Int_» W0 W1 = some _Val0)
+  (defn_Val1 : chop _Val0 = some _Val1)
+  (defn_Val2 : «_+Int_» PC_CELL 1 = some _Val2)
+  (defn_Val3 : «_<_>_SCHEDULE_Int_ScheduleConst_Schedule» SortScheduleConst.Gverylow_SCHEDULE_ScheduleConst SCHEDULE_CELL = some _Val3)
+  (defn_Val4 : «_-Int_» GAS_CELL _Val3 = some _Val4)
+  (req : USEGAS_CELL = true):
+  Rewrites
+    (@addLHS GAS_CELL PC_CELL W0 W1 K_CELL SCHEDULE_CELL USEGAS_CELL WS _DotVar0 _DotVar2 _Gen0 _Gen1 _Gen10 _Gen11 _Gen12 _Gen13 _Gen14 _Gen15 _Gen16 _Gen17 _Gen18 _Gen19 _Gen2 _Gen20 _Gen21 _Gen22 _Gen23 _Gen3 _Gen4 _Gen5 _Gen6 _Gen7 _Gen8 _Gen9)
+    (@addRHS _Val0 _Val1 _Val2 _Val4 K_CELL SCHEDULE_CELL WS _DotVar0 _DotVar2 _Gen0 _Gen1 _Gen10 _Gen11 _Gen12 _Gen13 _Gen14 _Gen15 _Gen16 _Gen17 _Gen18 _Gen19 _Gen2 _Gen20 _Gen21 _Gen22 _Gen23 _Gen3 _Gen4 _Gen5 _Gen6 _Gen7 _Gen8 _Gen9) := by
+  apply Rewrites.SUMMARY_ADD_2_SPEC_BASIC_BLOCK_8_TO_6 <;> try assumption
+
+theorem add_prestate_equiv
+  {GAS_CELL PC_CELL W0 W1 _Val0 _Val1 _Val2 _Val3 _Val4 : SortInt}
+  {K_CELL : SortK}
+  {SCHEDULE_CELL : SortSchedule}
+  {USEGAS_CELL : SortBool}
+  {WS : SortWordStack}
+  {_DotVar0 : SortGeneratedCounterCell}
+  {_DotVar2 : SortNetworkCell}
+  {_Gen0 : SortProgramCell}
+  {_Gen1 : SortJumpDestsCell}
+  {_Gen10 : SortCallDepthCell}
+  {_Gen11 : SortOutputCell}
+  {_Gen12 : SortStatusCodeCell}
+  {_Gen13 : SortCallStackCell}
+  {_Gen14 : SortInterimStatesCell}
+  {_Gen15 : SortTouchedAccountsCell}
+  {_Gen16 : SortVersionedHashesCell}
+  {_Gen17 : SortSubstateCell}
+  {_Gen18 : SortGasPriceCell}
+  {_Gen19 : SortOriginCell}
+  {_Gen2 : SortIdCell}
+  {_Gen20 : SortBlockhashesCell}
+  {_Gen21 : SortBlockCell}
+  {_Gen22 : SortExitCodeCell}
+  {_Gen23 : SortModeCell}
+  {_Gen3 : SortCallerCell}
+  {_Gen4 : SortCallDataCell}
+  {_Gen5 : SortCallValueCell}
+  {_Gen6 : SortLocalMemCell}
+  {_Gen7 : SortMemoryUsedCell}
+  {_Gen8 : SortCallGasCell}
+  {_Gen9 : SortStaticCell}
+  (symState : EVM.State):
+  stateMap symState (@addLHS GAS_CELL PC_CELL W0 W1 K_CELL SCHEDULE_CELL USEGAS_CELL WS _DotVar0 _DotVar2 _Gen0 _Gen1 _Gen10 _Gen11 _Gen12 _Gen13 _Gen14 _Gen15 _Gen16 _Gen17 _Gen18 _Gen19 _Gen2 _Gen20 _Gen21 _Gen22 _Gen23 _Gen3 _Gen4 _Gen5 _Gen6 _Gen7 _Gen8 _Gen9) =
+  {symState with
+    stack := (intMap W0) :: (intMap W1) :: wordStackMap WS
+    pc := intMap PC_CELL
+    gasAvailable := intMap GAS_CELL
+    executionEnv := {symState.executionEnv with code := _Gen0.val}
+    returnData := _Gen11.val
+    } := rfl
+
+theorem add_poststate_equiv
+  {PC_CELL W0 W1 _Val0 _Val1 _Val2 _Val3 _Val4 : SortInt}
+  {K_CELL : SortK}
+  {SCHEDULE_CELL : SortSchedule}
+  {WS : SortWordStack}
+  {_DotVar0 : SortGeneratedCounterCell}
+  {_DotVar2 : SortNetworkCell}
+  {_Gen0 : SortProgramCell}
+  {_Gen1 : SortJumpDestsCell}
+  {_Gen10 : SortCallDepthCell}
+  {_Gen11 : SortOutputCell}
+  {_Gen12 : SortStatusCodeCell}
+  {_Gen13 : SortCallStackCell}
+  {_Gen14 : SortInterimStatesCell}
+  {_Gen15 : SortTouchedAccountsCell}
+  {_Gen16 : SortVersionedHashesCell}
+  {_Gen17 : SortSubstateCell}
+  {_Gen18 : SortGasPriceCell}
+  {_Gen19 : SortOriginCell}
+  {_Gen2 : SortIdCell}
+  {_Gen20 : SortBlockhashesCell}
+  {_Gen21 : SortBlockCell}
+  {_Gen22 : SortExitCodeCell}
+  {_Gen23 : SortModeCell}
+  {_Gen3 : SortCallerCell}
+  {_Gen4 : SortCallDataCell}
+  {_Gen5 : SortCallValueCell}
+  {_Gen6 : SortLocalMemCell}
+  {_Gen7 : SortMemoryUsedCell}
+  {_Gen8 : SortCallGasCell}
+  {_Gen9 : SortStaticCell}
+  (defn_Val0 : «_+Int_» W0 W1 = some _Val0)
+  (defn_Val1 : chop _Val0 = some _Val1)
+  (defn_Val2 : «_+Int_» PC_CELL 1 = some _Val2)
+  (symState : EVM.State):
+  stateMap symState (@addRHS _Val0 _Val1 _Val2 _Val4 K_CELL SCHEDULE_CELL WS _DotVar0 _DotVar2 _Gen0 _Gen1 _Gen10 _Gen11 _Gen12 _Gen13 _Gen14 _Gen15 _Gen16 _Gen17 _Gen18 _Gen19 _Gen2 _Gen20 _Gen21 _Gen22 _Gen23 _Gen3 _Gen4 _Gen5 _Gen6 _Gen7 _Gen8 _Gen9) =
+  {symState with
+    stack := (intMap (chop' («_+Int'_» W0 W1))) :: wordStackMap WS
+    pc := intMap («_+Int'_» PC_CELL 1)
+    gasAvailable := intMap _Val4
+    executionEnv := {symState.executionEnv with code := _Gen0.val}
+    returnData := _Gen11.val
+    } := by aesop (add simp [«_+Int'_», chop'])
+
+open AddSummary
+
+-- We cannot prove full equivalence for the `EVM.step` function
+-- This is because it doesn't include all semantics such as gas computation
+theorem step_add_equiv
+  {GAS_CELL PC_CELL W0 W1 _Val0 _Val1 _Val2 _Val3 _Val4 : SortInt}
+  {K_CELL : SortK}
+  {SCHEDULE_CELL : SortSchedule}
+  {USEGAS_CELL : SortBool}
+  {WS : SortWordStack}
+  {_DotVar0 : SortGeneratedCounterCell}
+  {_DotVar2 : SortNetworkCell}
+  {_Gen0 : SortProgramCell}
+  {_Gen1 : SortJumpDestsCell}
+  {_Gen10 : SortCallDepthCell}
+  {_Gen11 : SortOutputCell}
+  {_Gen12 : SortStatusCodeCell}
+  {_Gen13 : SortCallStackCell}
+  {_Gen14 : SortInterimStatesCell}
+  {_Gen15 : SortTouchedAccountsCell}
+  {_Gen16 : SortVersionedHashesCell}
+  {_Gen17 : SortSubstateCell}
+  {_Gen18 : SortGasPriceCell}
+  {_Gen19 : SortOriginCell}
+  {_Gen2 : SortIdCell}
+  {_Gen20 : SortBlockhashesCell}
+  {_Gen21 : SortBlockCell}
+  {_Gen22 : SortExitCodeCell}
+  {_Gen23 : SortModeCell}
+  {_Gen3 : SortCallerCell}
+  {_Gen4 : SortCallDataCell}
+  {_Gen5 : SortCallValueCell}
+  {_Gen6 : SortLocalMemCell}
+  {_Gen7 : SortMemoryUsedCell}
+  {_Gen8 : SortCallGasCell}
+  {_Gen9 : SortStaticCell}
+  (defn_Val0 : «_+Int_» W0 W1 = some _Val0)
+  (defn_Val1 : chop _Val0 = some _Val1)
+  (defn_Val2 : «_+Int_» PC_CELL 1 = some _Val2)
+  (defn_Val3 : «_<_>_SCHEDULE_Int_ScheduleConst_Schedule» SortScheduleConst.Gverylow_SCHEDULE_ScheduleConst SCHEDULE_CELL = some _Val3)
+  (defn_Val4 : «_-Int_» GAS_CELL _Val3 = some _Val4)
+  (symState : EVM.State)
+  -- needed for EVM.step
+  (gas gasCost : ℕ)
+  -- Necessary assumptions for equivalence
+  (cancun : SCHEDULE_CELL = .CANCUN_EVM)
+  (gasEnough : 0 < gas)
+  (gavailEnough : 3 ≤ GAS_CELL)
+  (gavailSmall : GAS_CELL < ↑UInt256.size)
+  (gasCostValue : gasCost = GasConstants.Gverylow)
+  (pcountSmall : PC_CELL + 1 < UInt256.size)
+  (pcountNonneg : 0 ≤ PC_CELL)
+  (W0ge0 : 0 ≤ W0)
+  (W1ge0 : 0 ≤ W1):
+  EVM.step_add gas gasCost (stateMap symState (@addLHS GAS_CELL PC_CELL W0 W1 K_CELL SCHEDULE_CELL USEGAS_CELL WS _DotVar0 _DotVar2 _Gen0 _Gen1 _Gen10 _Gen11 _Gen12 _Gen13 _Gen14 _Gen15 _Gen16 _Gen17 _Gen18 _Gen19 _Gen2 _Gen20 _Gen21 _Gen22 _Gen23 _Gen3 _Gen4 _Gen5 _Gen6 _Gen7 _Gen8 _Gen9)) =
+  .ok (stateMap {symState with execLength := symState.execLength + 1} (@addRHS _Val0 _Val1 _Val2 _Val4 K_CELL SCHEDULE_CELL WS _DotVar0 _DotVar2 _Gen0 _Gen1 _Gen10 _Gen11 _Gen12 _Gen13 _Gen14 _Gen15 _Gen16 _Gen17 _Gen18 _Gen19 _Gen2 _Gen20 _Gen21 _Gen22 _Gen23 _Gen3 _Gen4 _Gen5 _Gen6 _Gen7 _Gen8 _Gen9)) := by
+  rw [add_prestate_equiv, add_poststate_equiv] <;> try assumption
+  cases gas; contradiction
+  case succ gas =>
+    rw [EVM.step_add_summary] <;> try assumption
+    congr
+    . aesop (add simp [GasInterface.cancun_def, «_-Int_», intMap_sub_dist])
+    . rw [plusInt_def, ←UInt256.add_succ_mod_size, intMap_add_dist] <;> aesop
+    . aesop (add simp [intMap, chop_def, plusInt_def, intMap_add_dist])
+
+/- Deviations from the KEVM produced specifications:
+ 1. The program is not symbolic, it is instead a 1-opcode (`ADD`) program
+ 2. The program counter is also not symbolic, and it is set to 0
+ 3. In the RHS, the output cell (mapped to `returnData`) is set to `ByteArray.empty`
+ 4. The schedule is set to `CANCUN`
+ 5. `GAVAIL` is in the `UInt256` range
+ 6. `W0` and `W1` are nonnegative
+ -/
+theorem X_add_equiv
+  {GAS_CELL PC_CELL W0 W1 _Val0 _Val1 _Val2 _Val3 _Val4 : SortInt}
+  {K_CELL : SortK}
+  {SCHEDULE_CELL : SortSchedule}
+  {USEGAS_CELL : SortBool}
+  {WS : SortWordStack}
+  {_DotVar0 : SortGeneratedCounterCell}
+  {_DotVar2 : SortNetworkCell}
+  {_Gen0 : SortProgramCell}
+  {_Gen1 : SortJumpDestsCell}
+  {_Gen10 : SortCallDepthCell}
+  {_Gen11 : SortOutputCell}
+  {_Gen12 : SortStatusCodeCell}
+  {_Gen13 : SortCallStackCell}
+  {_Gen14 : SortInterimStatesCell}
+  {_Gen15 : SortTouchedAccountsCell}
+  {_Gen16 : SortVersionedHashesCell}
+  {_Gen17 : SortSubstateCell}
+  {_Gen18 : SortGasPriceCell}
+  {_Gen19 : SortOriginCell}
+  {_Gen2 : SortIdCell}
+  {_Gen20 : SortBlockhashesCell}
+  {_Gen21 : SortBlockCell}
+  {_Gen22 : SortExitCodeCell}
+  {_Gen23 : SortModeCell}
+  {_Gen3 : SortCallerCell}
+  {_Gen4 : SortCallDataCell}
+  {_Gen5 : SortCallValueCell}
+  {_Gen6 : SortLocalMemCell}
+  {_Gen7 : SortMemoryUsedCell}
+  {_Gen8 : SortCallGasCell}
+  {_Gen9 : SortStaticCell}
+  (defn_Val0 : «_+Int_» W0 W1 = some _Val0)
+  (defn_Val1 : chop _Val0 = some _Val1)
+  (defn_Val2 : «_+Int_» PC_CELL 1 = some _Val2)
+  (defn_Val3 : «_<_>_SCHEDULE_Int_ScheduleConst_Schedule» SortScheduleConst.Gverylow_SCHEDULE_ScheduleConst SCHEDULE_CELL = some _Val3)
+  (defn_Val4 : «_-Int_» GAS_CELL _Val3 = some _Val4)
+  (symState : EVM.State)
+  -- Necessary assumptions for equivalence
+  (cancun : SCHEDULE_CELL = .CANCUN_EVM)
+  (codeAdd : _Gen0 = ⟨⟨#[(1 : UInt8)]⟩⟩)
+  (pcZero : PC_CELL = 0)
+  (enoughGas : 3 < GAS_CELL)
+  (boundedGas : GAS_CELL < ↑UInt256.size)
+  (W0ge0 : 0 ≤ W0)
+  (W1ge0 : 0 ≤ W1)
+  -- There's no #sizeWordStack
+  (wordStackOk : sizeWordStackAux WS 0 < some 1024):
+  EVM.X false (UInt256.toNat (intMap GAS_CELL)) (stateMap symState (@addLHS GAS_CELL PC_CELL W0 W1 K_CELL SCHEDULE_CELL USEGAS_CELL WS _DotVar0 _DotVar2 _Gen0 _Gen1 _Gen10 _Gen11 _Gen12 _Gen13 _Gen14 _Gen15 _Gen16 _Gen17 _Gen18 _Gen19 _Gen2 _Gen20 _Gen21 _Gen22 _Gen23 _Gen3 _Gen4 _Gen5 _Gen6 _Gen7 _Gen8 _Gen9)) =
+  .ok (.success (stateMap {symState with execLength := symState.execLength + 2} (@addRHS _Val0 _Val1 _Val2 _Val4 K_CELL SCHEDULE_CELL WS _DotVar0 _DotVar2 _Gen0 _Gen1 _Gen10 ⟨ByteArray.empty⟩ _Gen12 _Gen13 _Gen14 _Gen15 _Gen16 _Gen17 _Gen18 _Gen19 _Gen2 _Gen20 _Gen21 _Gen22 _Gen23 _Gen3 _Gen4 _Gen5 _Gen6 _Gen7 _Gen8 _Gen9)) ByteArray.empty) := by
+  -- With `simp` doesn't work
+  rw [codeAdd, pcZero, add_prestate_equiv, add_poststate_equiv] <;> try assumption
+  -- If we don't apply this lemma we cannot rewrite X_add_summary
+  have pc_equiv : intMap 0 = UInt256.ofNat 0 := rfl
+  rw [pc_equiv, X_add_summary]
+  · aesop (add simp [GasInterface.cancun_def, «_-Int_», chop_def, plusInt_def, intMap_add_dist])
+      (add safe (by rw [intMap_sub_dist])) (add safe (by apply le_of_lt))
+  · aesop (add simp [GasConstants.Gverylow, intMap, UInt256.toSigned])
+      (add simp [intMap_toNat, UInt256.ofNat_toNat])
+      (add safe (by contradiction))
+  · simp_all [sizeWordStack_def]
+    simp [LT.lt, Option.lt, OfNat.ofNat, (@Int.ofNat_eq_coe 1024)] at wordStackOk
+    exact (Int.lt_of_ofNat_lt_ofNat wordStackOk)
+
+end AddOpcodeEquivalence
