EvmEquivalence/Interfaces/EvmYulInterface.lean
@@ -1,6 +1,10 @@
-import EvmYul.UInt256
+import EvmYul.EVM.Semantics
+import EvmEquivalence.Summaries.StopSummary
+import EvmEquivalence.Utils.IntUtils
+
 
 open EvmYul
+open EVM
 
 namespace UInt256
 
@@ -8,7 +12,8 @@ section
 
 set_option linter.deprecated false
 
-  variable {n : ℕ}
+variable {n : ℕ}
+variable {p : ℤ}
 
 theorem val_eq (h : n < UInt256.size): ↑(UInt256.ofNat n).1 = n := by
   aesop (add simp [UInt256.ofNat, Id.run, Fin.ofNat])
@@ -17,11 +22,62 @@ theorem val_eq (h : n < UInt256.size): ↑(UInt256.ofNat n).1 = n := by
 theorem ofNat_eq: UInt256.ofNat n = ⟨Fin.ofNat n⟩ := by
   aesop (add simp [UInt256.ofNat])
 
-theorem ofNat_toNat (h : n < UInt256.size): (UInt256.ofNat n).toNat = n := by
-  have le_fls : (UInt256.size ≤ n) = False := by aesop
-  simp [UInt256.ofNat, Id.run, Fin.ofNat, UInt256.toNat]; split <;> try simp_all
-  simp_all [UInt256.size]
+theorem ofNat_toNat (n_le_size : n < UInt256.size) :
+  (UInt256.ofNat n).toNat = n := by
+  aesop (add simp [UInt256.ofNat, UInt256.toNat, Id.run, dbgTrace, Fin.ofNat])
+
+@[simp]
+theorem sub_0 {n : UInt256} : n - .ofNat 0 = n := by
+  match n with
+  | UInt256.mk (Fin.mk val isLT) =>
+  simp [UInt256.ofNat, Id.run, HSub.hSub, Sub.sub, UInt256.sub]
+  simp [UInt256.size, Fin.ofNat, Fin.sub]; assumption
+  -- Alternatively:
+  /- simp [UInt256.ofNat]; split; try contradiction
+  simp [Id.run, HSub.hSub, Sub.sub, UInt256.sub]
+  simp [Fin.sub]; rw [Nat.mod_eq_iff_lt]; assumption; simp [UInt256.size] -/
+
+@[simp]
+theorem zero_add: .ofNat 0 + .ofNat n = UInt256.ofNat n := by
+  simp [UInt256.ofNat, Id.run, dbgTrace, Fin.ofNat, HAdd.hAdd]
+  simp [Add.add, UInt256.add, Fin.add_def]
+
+theorem add_succ_mod_size (pos : 0 ≤ p) (size_ok : p + 1 < UInt256.size) : (p + 1) % UInt256.size = p + 1 := by
+        rw [Int.mod_cast, Int.toNat_ofNat, Nat.mod_eq_of_lt] <;> aesop (add safe (by omega))
 
 end
 
 end UInt256
+
+@[simp]
+theorem isCreate_false {τ : OperationType} (opcode : Operation τ) (noCreate : opcode ≠ Operation.CREATE) (noCreate2 : opcode ≠ Operation.CREATE2):
+  opcode.isCreate = false := by
+  cases opc: opcode <;> rw [Operation.isCreate]; next op =>
+  cases op <;> aesop
+
+section
+
+variable {gas gasCost : ℕ}
+
+/--
+Execution result of `X` for a single-opcode program when `pc` is set to 1
+ -/
+theorem X_bad_pc {opcode : UInt8}
+                 {symState : EVM.State}
+                 (gpos : 1 < gas)
+                 (pc1 : symState.pc = .ofNat 1)
+                 (opcode_single : symState.executionEnv.code = ⟨#[opcode]⟩)
+                 (stack_ok : symState.stack.length < 1025):
+  X false gas symState =
+  Except.ok (.success {symState with
+      returnData := ByteArray.empty,
+      execLength := symState.execLength + 1} ByteArray.empty) := by
+  cases cgas: gas; rw [cgas] at gpos; contradiction
+  simp_all [X, δ, α]; split; aesop (add safe (by contradiction)) (add safe (by linarith))
+  dsimp [Except.instMonad, Except.bind]; rename_i n _ _ _ heq
+  revert heq; split; aesop (add safe (by contradiction)) (add safe (by linarith))
+  simp [pure, Except.pure]; intro evm_eq cost; subst evm_eq cost
+  cases n; contradiction
+  simp [StopSummary.EVM.step_stop_summary_simple]
+
+end
