EvmEquivalence/Summaries/Push0Summary.lean
@@ -1,0 +1,115 @@
+import EvmYul.EVM.Semantics
+import EvmYul.EVM.GasConstants
+import EvmEquivalence.Interfaces.EvmYulInterface
+import EvmEquivalence.Summaries.StopSummary
+
+open EvmYul
+open EVM
+
+namespace Push0Summary
+
+section
+
+variable (gas gasCost : ℕ)
+variable (symStack : Stack UInt256)
+variable (symPc : UInt256)
+variable (symGasAvailable : UInt256)
+variable (symExecLength : ℕ)
+variable (symReturnData symCode : ByteArray)
+
+@[simp]
+abbrev push0EVM := @Operation.PUSH0
+
+@[simp]
+abbrev push0_instr : Option (Operation .EVM × Option (UInt256 × Nat)) :=
+  some ⟨push0EVM, none⟩
+
+@[simp]
+def EVM.step_push0 : Transformer :=
+  EVM.step false gas gasCost push0_instr
+
+@[simp]
+def EvmYul.step_push0 : Transformer :=
+  @EvmYul.step OperationType.EVM false push0EVM
+
+theorem EvmYul.step_push0_summary (symState : EVM.State):
+  EvmYul.step_push0 {symState with
+    stack := symStack,
+    pc := symPc} = default := rfl
+
+theorem EVM.step_push0_summary_simple (gpos : 0 < gas) (symState : EVM.State):
+  @EVM.step_push0 gas gasCost symState =
+    .ok {symState with
+    stack := (.ofNat 0) :: symState.stack
+    gasAvailable := symState.gasAvailable - UInt256.ofNat gasCost
+    pc := symState.pc + .ofNat 1,
+    execLength := symState.execLength + 1} := by
+  cases gas; contradiction; rfl
+
+theorem EVM.step_push0_summary (gpos : 0 < gas) (symState : EVM.State):
+  @EVM.step_push0 gas gasCost
+    {symState with
+      stack := symStack,
+      pc := symPc,
+      gasAvailable := symGasAvailable,
+      execLength := symExecLength,
+      executionEnv := {symState.executionEnv with code := symCode},
+      returnData := symReturnData} =
+    .ok {symState with
+    stack := (.ofNat 0) :: symStack
+    gasAvailable := symGasAvailable - UInt256.ofNat gasCost
+    pc := symPc + .ofNat 1,
+    executionEnv := {symState.executionEnv with code := symCode},
+    returnData := symReturnData,
+    execLength := symExecLength + 1} := by
+  cases gas; contradiction; rfl
+
+@[simp]
+theorem decode_singleton_push0 :
+  decode ⟨#[0x5F]⟩ (.ofNat 0) = some ⟨push0EVM, none⟩ := rfl
+
+@[simp]
+theorem memoryExpansionCost_push0 (symState : EVM.State) :
+  memoryExpansionCost symState push0EVM = 0 := by
+  simp [memoryExpansionCost, memoryExpansionCost.μᵢ']
+
+@[simp]
+theorem C'_push0 (symState : EVM.State) :
+  C' symState push0EVM = GasConstants.Gbase := by rfl
+
+theorem X_push0_summary (enoughGas : GasConstants.Gbase < symGasAvailable.toNat)
+                      (symStack_ok : symStack.length < 1024)
+                      (symState : EVM.State):
+  X false symGasAvailable.toNat
+  {symState with
+    stack := symStack,
+    pc := .ofNat 0,
+    execLength := symExecLength,
+    gasAvailable := symGasAvailable,
+    executionEnv := {symState.executionEnv with code := ⟨#[(0x5F : UInt8)]⟩}
+    returnData := symReturnData} =
+  Except.ok (.success {symState with
+        stack := (.ofNat 0) :: symStack,
+        pc := .ofNat 1,
+        gasAvailable := symGasAvailable - .ofNat GasConstants.Gbase,
+        executionEnv := {symState.executionEnv with code := ⟨#[(0x5F : UInt8)]⟩},
+        returnData := ByteArray.empty,
+        execLength := symExecLength + 2} ByteArray.empty):= by
+  cases g_case: symGasAvailable.toNat; rw [g_case] at enoughGas; contradiction
+  case succ g_pos =>
+  have enough_gas_rw : (symGasAvailable.toNat < GasConstants.Gbase) = False :=
+    by aesop (add safe (by omega))
+  have stack_ok_rw : (1024 < List.length symStack + (α push0EVM).getD 0) = False :=
+    by simp [α]; omega
+  have gPos : (0 < g_pos) := by aesop (add simp [GasConstants.Gbase]) (add safe (by omega))
+  simp [X, δ, enough_gas_rw, stack_ok_rw]; split; contradiction
+  rename_i evm _ stateOk; revert stateOk
+  simp [pure, Except.pure]; intro evm_eq cost; subst cost evm_eq
+  dsimp [Except.instMonad, Except.bind]
+  have step_rw := (@EVM.step_push0_summary g_pos GasConstants.Gbase symStack (.ofNat 0) symGasAvailable symExecLength symReturnData ⟨#[(0x5F : UInt8)]⟩ gPos)
+  rw [EVM.step_push0, push0_instr] at step_rw; simp [step_rw]
+  rw [X_bad_pc] <;> aesop (add simp [GasConstants.Gbase]) (add safe (by omega))
+
+end
+
+end Push0Summary
